pulse/share/steel/examples/pulse/dice/Array.fst
@@ -1,0 +1,80 @@
+module Array
+module A = Steel.ST.Array
+module R = Steel.ST.Reference
+module PM = Pulse.Main
+open Steel.ST.Array
+open Steel.FractionalPermission
+open Steel.ST.Util
+open FStar.Ghost
+open Pulse.Steel.Wrapper
+module US = FStar.SizeT
+module U8 = FStar.UInt8
+
+let elseq (a:Type) (l:nat) = s:Ghost.erased (Seq.seq a) { Seq.length s == l }
+
+```pulse
+fn compare (#t:eqtype) (l:US.t) (a1 a2:A.larray t (US.v l))
+           (#p1 #p2:perm) (#s1 #s2:elseq t (US.v l))
+  requires (
+    A.pts_to a1 p1 s1 `star`
+    A.pts_to a2 p2 s2
+  )
+  returns res:bool
+  ensures (
+    A.pts_to a1 p1 s1 `star`
+    A.pts_to a2 p2 s2 `star`
+    (pure (res <==> Seq.equal s1 s2))
+  )
+{
+  let mut i = 0sz;
+  while (let vi = !i; if US.(vi <^ l) { let v1 = a1.(vi); let v2 = a2.(vi); (v1 = v2) } else { false } )
+  invariant b. exists (vi:US.t). ( 
+    R.pts_to i full_perm vi `star`
+    A.pts_to a1 p1 s1 `star`
+    A.pts_to a2 p2 s2 `star`
+    pure (
+      US.v vi <= US.v l /\
+      (b == (US.(vi <^ l) && Seq.index s1 (US.v vi) = Seq.index s2 (US.v vi))) /\
+      (forall (i:nat). i < US.v vi ==> Seq.index s1 i == Seq.index s2 i)
+    )
+  )
+  {
+    let vi = !i; 
+    i := US.(vi +^ 1sz);
+    ()
+  };
+  let vi = !i;
+  let res = vi = l;
+  res
+}
+```
+
+```pulse
+fn fill_array (#t:Type0) (l:US.t) (a:(a:A.array t{ US.v l == A.length a })) (v:t)
+              (#s:(s:Ghost.erased (Seq.seq t) { Seq.length s == US.v l }))
+   requires (A.pts_to a full_perm s)
+   ensures 
+      exists (s:Seq.seq t). (
+         A.pts_to a full_perm s `star`
+         pure (s `Seq.equal` Seq.create (US.v l) v)
+      )
+{
+   let mut i = 0sz;
+   while (let vi = !i; US.(vi <^ l))
+   invariant b. exists (s:Seq.seq t) (vi:US.t). ( 
+      A.pts_to a full_perm s `star`
+      R.pts_to i full_perm vi `star`
+      pure ((b == US.(vi <^ l)) /\
+            US.v vi <= US.v l /\
+            Seq.length s == A.length a /\
+            (forall (i:nat). i < US.v vi ==> Seq.index s i == v))
+   )
+   {
+      let vi = !i; 
+      (a.(vi) <- v);
+      i := US.(vi +^ 1sz);
+      ()
+   };
+   ()
+}
+```
